finish progress

SystemFD/Metatheory/Canonicity.lean
@@ -82,24 +82,24 @@ cases tJ; case _ wf h1 =>
   case _ =>
     injection h1 with h1; cases h1;
     have lem := ctx_get_var_type wf fh;
-    sorry
-    -- have uniq := uniqueness_of_kinds tstar lem;
-    -- cases uniq;
+    have lem1 := kind_shape lem rfl
+    have lem2 := type_shape tstar (by constructor)
+    exfalso; apply Term.is_kind_disjoint_is_type lem1 lem2
   case _ =>
     injection h1 with h1; cases h1;
     have lem := ctx_get_datatype_kind wf fh;
-    sorry
-    -- have uniq := uniqueness_of_kinds tstar lem;
-    -- cases uniq;
+    have lem1 := kind_shape lem rfl
+    have lem2 := type_shape tstar (by constructor)
+    exfalso; apply Term.is_kind_disjoint_is_type lem1 lem2
   case _ =>
       cases h1; apply Or.inl;
       unfold Ctx.is_ctor; unfold Frame.is_ctor; rw [fh]
   case _ =>
     injection h1 with h1; cases h1;
     have lem := ctx_get_opent_kind wf fh;
-    sorry
-    -- have uniq := uniqueness_of_kinds tstar lem;
-    -- cases uniq;
+    have lem1 := kind_shape lem rfl
+    have lem2 := type_shape tstar (by constructor)
+    exfalso; apply Term.is_kind_disjoint_is_type lem1 lem2
   case _ =>
     cases h1; apply Or.inr;
     unfold Ctx.is_insttype; unfold Frame.is_insttype; rw[fh]
@@ -110,51 +110,63 @@ theorem cannonical_head :
   Γ ⊢ τ : ★ ->
   t.neutral_form = .some (h, ts) ->
   (Γ.is_ctor h ∨ Γ.is_insttype h)
-:= by sorry
--- intro vt tJ τJ tnf;
--- have tshape := Term.neutral_form_law (Eq.symm tnf)
--- rw[<-tshape] at tJ;
--- have hJ := inversion_apply_spine tJ;
--- cases hJ; case _ τ' hJ =>
--- cases hJ; case _ spTy hJ =>
--- cases vt;
--- any_goals(solve | cases tnf)
--- case app h_stable tnf' =>
---   rw[tnf] at tnf'; cases tnf';
---   cases hJ; case _ wf gt =>
---   have τ'J := spine_type_is_type τJ spTy
---   have hJ := Judgment.var wf gt;
---   simp at h_stable;
---   generalize fh : Γ d@ h = f at *;
---   cases f;
---   any_goals (solve | cases gt)
---   all_goals (unfold Frame.is_stable_red at h_stable; simp at h_stable)
---   all_goals (clear h_stable; unfold Frame.get_type at gt; simp at gt; cases gt)
---   repeat sorry
-  -- case _ =>
-  --   have h := ctx_get_var_type wf fh;
-  --   have uniq := uniqueness_of_types h τ'J; cases uniq;
-  -- case _ =>
-  --   have h := ctx_get_datatype_kind wf fh;
-  --   have uniq := uniqueness_of_types h τ'J; cases uniq;
-  -- case _ =>
-  --   apply Or.inl;
-  --   simp; rw[fh]; unfold Frame.is_ctor; simp;
-  -- case _ =>
-  --   have h := ctx_get_opent_kind wf fh
-  --   have uniq := uniqueness_of_types h τ'J; cases uniq;
-  -- case _ =>
-  --   apply Or.inr;
-  --   simp; rw[fh]; unfold Frame.is_insttype; simp;
+:= by
+intro vt tJ τJ tnf;
+have tshape := Term.neutral_form_law (Eq.symm tnf)
+rw[<-tshape] at tJ;
+have hJ := inversion_apply_spine tJ;
+cases hJ; case _ τ' hJ =>
+cases hJ; case _ spTy hJ =>
+cases hJ; case _ hJ h3 =>
+cases vt;
+any_goals(solve | cases tnf)
+case app h_stable tnf' =>
+  rw[tnf] at tnf'; cases tnf';
+  cases hJ; case _ wf gt =>
+  have τ'J := spine_type_is_type τJ spTy
+  have hJ := Judgment.var wf gt;
+  simp at h_stable;
+  generalize fh : Γ d@ h = f at *;
+  cases f;
+  any_goals (solve | cases gt)
+  all_goals (unfold Frame.is_stable_red at h_stable; simp at h_stable)
+  all_goals (clear h_stable; unfold Frame.get_type at gt; simp at gt; cases gt)
+  case _ =>
+    have h := ctx_get_var_type wf fh;
+    have lem1 := kind_shape h rfl
+    have lem2 := type_shape τ'J (by constructor)
+    exfalso; apply Term.is_kind_disjoint_is_type lem1 lem2
+  case _ =>
+    have h := ctx_get_datatype_kind wf fh;
+    have lem1 := kind_shape h rfl
+    have lem2 := type_shape τ'J (by constructor)
+    exfalso; apply Term.is_kind_disjoint_is_type lem1 lem2
+  case _ =>
+    apply Or.inl;
+    simp; rw[fh]; unfold Frame.is_ctor; simp;
+  case _ =>
+    have h := ctx_get_opent_kind wf fh
+    have lem1 := kind_shape h rfl
+    have lem2 := type_shape τ'J (by constructor)
+    exfalso; apply Term.is_kind_disjoint_is_type lem1 lem2
+  case _ =>
+    apply Or.inr;
+    simp; rw[fh]; unfold Frame.is_insttype; simp;
 
 
 inductive ArrowLike : (T : Term) -> Prop where
 | arrowt : ArrowLike (A -t> B)
 | allt : ArrowLike (∀[A] B)
 
-inductive LambdaLike : (T : Term) -> Prop where
-| lam : LambdaLike (`λ[A] B)
-| lamt : LambdaLike (Λ[A] B)
+inductive LambdaLike (Γ : Ctx Term) : (T : Term) -> Prop where
+| lam : LambdaLike Γ (`λ[A] B)
+| lamt : LambdaLike Γ (Λ[A] B)
+| ctor : ValidHeadVariable t Γ.is_ctor -> LambdaLike Γ t
+| insttype : ValidHeadVariable t Γ.is_insttype -> LambdaLike Γ t
+| choice :
+  LambdaLike Γ t1 ->
+  LambdaLike Γ t2 ->
+  LambdaLike Γ (t1 ⊕ t2)
 
 @[simp]
 abbrev CanonicalLambdaType (Γ : Ctx Term) : (v : JudgmentVariant) -> JudgmentArgs v -> Prop
@@ -163,191 +175,199 @@ abbrev CanonicalLambdaType (Γ : Ctx Term) : (v : JudgmentVariant) -> JudgmentAr
        Γ ⊢ t : τ ->
        Γ ⊢ τ : ★ ->
        ArrowLike τ ->
-       (LambdaLike t ∨ ValidHeadVariable t Γ.is_ctor ∨ ValidHeadVariable t Γ.is_insttype)
+       LambdaLike Γ t
 | .wf => λ () => true
 
 theorem canonical_lambda :
   Judgment v Γ idx ->
   CanonicalLambdaType Γ v idx
-:= by sorry
--- intro j; induction j <;> simp at *
--- all_goals (intro h1 h2 h3 h4)
--- any_goals try (solve | cases h1; case _ h1 => cases h1)
--- any_goals try (solve | cases h3)
--- case _ Γ n T wf gt ih =>
---   cases h1; case _ n_stable nnf =>
---   simp at nnf; cases nnf; case _ e1 e2 =>
---   subst e1; subst e2;
---   generalize fh : Γ d@ n = f at *;
---   unfold Frame.get_type at gt;
---   cases h4;
---   case _ =>
---     split at gt;
---     any_goals (solve | cases gt)
---     any_goals (solve | unfold Ctx.is_stable_red at n_stable; unfold Frame.is_stable_red at n_stable;
---                        exfalso; rw[fh] at n_stable; simp at n_stable)
---     all_goals (cases gt)
---     case _ =>
---       have lem := classification_lemma h3; simp at lem;
---       cases lem;
---       case _ =>
---         have wfr := @frame_wf_by_index Γ n wf;
---         have h := ctx_get_var_type wf fh;
---         cases h
---       case _ h =>
---         cases h; case _ k h => cases h; case _ _ h => cases h; case _ h => cases h
---     case _ =>
---       have wfr := @frame_wf_by_index Γ n wf;
---       have h := ctx_get_datatype_kind wf fh;
---       cases h;
---     case _ =>
---       apply Or.inr; apply Or.inl; unfold ValidHeadVariable;
---       apply Exists.intro (n, []);
---       apply And.intro; simp; simp; rw[fh]; unfold Frame.is_ctor; simp
---     case _ =>
---       have wfr := @frame_wf_by_index Γ n wf;
---       have h := ctx_get_opent_kind wf fh;
---       cases h;
---     case _ =>
---       apply Or.inr; apply Or.inr; unfold ValidHeadVariable;
---       apply Exists.intro (n, []);
---       apply And.intro; simp; simp; rw[fh]; unfold Frame.is_insttype; simp
---   case _ =>
---     split at gt;
---     any_goals (solve | cases gt)
---     any_goals (solve | unfold Ctx.is_stable_red at n_stable; unfold Frame.is_stable_red at n_stable;
---                        exfalso; rw[fh] at n_stable; simp at n_stable)
---     all_goals (cases gt)
---     case _ =>
---       have lem := classification_lemma h3; simp at lem;
---       cases lem;
---       case _ =>
---         have wfr := @frame_wf_by_index Γ n wf;
---         have h := ctx_get_var_type wf fh;
---         cases h
---       case _ h =>
---         cases h; case _ k h => cases h; case _ _ h => cases h; case _ h => cases h
---     case _ =>
---       have wfr := @frame_wf_by_index Γ n wf;
---       have h := ctx_get_datatype_kind wf fh;
---       cases h;
---     case _ =>
---       apply Or.inr; apply Or.inl; unfold ValidHeadVariable;
---       apply Exists.intro (n, []);
---       apply And.intro; simp; simp; rw[fh]; unfold Frame.is_ctor; simp
---     case _ =>
---       have wfr := @frame_wf_by_index Γ n wf;
---       have h := ctx_get_opent_kind wf fh;
---       cases h;
---     case _ =>
---       apply Or.inr; apply Or.inr; unfold ValidHeadVariable;
---       apply Exists.intro (n, []);
---       apply And.intro; simp; simp; rw[fh]; unfold Frame.is_insttype; simp
+:= by
+intro j; induction j <;> simp at *
+all_goals (intro h1 h2 h3 h4)
+any_goals try (solve | cases h1; case _ h1 => cases h1)
+any_goals try (solve | cases h3)
+case _ Γ n T wf gt ih =>
+  cases h1; case _ n_stable nnf =>
+  simp at nnf; cases nnf; case _ e1 e2 =>
+  subst e1; subst e2;
+  generalize fh : Γ d@ n = f at *;
+  unfold Frame.get_type at gt;
+  cases h4;
+  case _ =>
+    split at gt;
+    any_goals (solve | cases gt)
+    any_goals (solve | unfold Ctx.is_stable_red at n_stable; unfold Frame.is_stable_red at n_stable;
+                       exfalso; rw[fh] at n_stable; simp at n_stable)
+    all_goals (cases gt)
+    case _ =>
+      have lem := classification_lemma h3; simp at lem;
+      cases lem;
+      case _ =>
+        have wfr := @frame_wf_by_index Γ n wf;
+        have h := ctx_get_var_type wf fh;
+        cases h
+      case _ h =>
+        cases h; case _ k h => cases h; case _ _ h => cases h; case _ h => cases h
+    case _ =>
+      have wfr := @frame_wf_by_index Γ n wf;
+      have h := ctx_get_datatype_kind wf fh;
+      cases h;
+    case _ =>
+      apply LambdaLike.ctor; unfold ValidHeadVariable;
+      apply Exists.intro (n, []);
+      apply And.intro; simp; simp; rw[fh]; unfold Frame.is_ctor; simp
+    case _ =>
+      have wfr := @frame_wf_by_index Γ n wf;
+      have h := ctx_get_opent_kind wf fh;
+      cases h;
+    case _ =>
+      apply LambdaLike.insttype; unfold ValidHeadVariable;
+      apply Exists.intro (n, []);
+      apply And.intro; simp; simp; rw[fh]; unfold Frame.is_insttype; simp
+  case _ =>
+    split at gt;
+    any_goals (solve | cases gt)
+    any_goals (solve | unfold Ctx.is_stable_red at n_stable; unfold Frame.is_stable_red at n_stable;
+                       exfalso; rw[fh] at n_stable; simp at n_stable)
+    all_goals (cases gt)
+    case _ =>
+      have lem := classification_lemma h3; simp at lem;
+      cases lem;
+      case _ =>
+        have wfr := @frame_wf_by_index Γ n wf;
+        have h := ctx_get_var_type wf fh;
+        cases h
+      case _ h =>
+        cases h; case _ k h => cases h; case _ _ h => cases h; case _ h => cases h
+    case _ =>
+      have wfr := @frame_wf_by_index Γ n wf;
+      have h := ctx_get_datatype_kind wf fh;
+      cases h;
+    case _ =>
+      apply LambdaLike.ctor; unfold ValidHeadVariable;
+      apply Exists.intro (n, []);
+      apply And.intro; simp; simp; rw[fh]; unfold Frame.is_ctor; simp
+    case _ =>
+      have wfr := @frame_wf_by_index Γ n wf;
+      have h := ctx_get_opent_kind wf fh;
+      cases h;
+    case _ =>
+      apply LambdaLike.insttype; unfold ValidHeadVariable;
+      apply Exists.intro (n, []);
+      apply And.intro; simp; simp; rw[fh]; unfold Frame.is_insttype; simp
 
--- case _ Γ f _ _ _ fJ _ _ ih => -- appk bogus case
---   cases h1; case _ n ts n_stable ts' =>
---   simp at ts'; rw [Option.bind_eq_some] at ts';  cases ts'; case _ w fnf =>
---   cases fnf; case _ fnf ts' =>
---   cases ts';
---   have vf : Val Γ f := by constructor; assumption; assumption
---   generalize fh : Γ d@ w.fst = f at *;
---   have lem := classification_lemma fJ; simp at lem; cases lem;
---   case _ h => cases h; case _ k1 k2 => sorry
---     -- have h := uniqueness_of_types h3 k2; cases h;
---   case _ h =>
---     cases h; case _ w h =>
---     cases h; case _ wk arrk =>
---     cases arrk; cases wk;
+case _ Γ f _ _ _ fJ _ _ ih => -- appk bogus case
+  cases h1; case _ n ts n_stable ts' =>
+  simp at ts'; rw [Option.bind_eq_some] at ts';  cases ts'; case _ w fnf =>
+  cases fnf; case _ fnf ts' =>
+  cases ts';
+  have vf : Val Γ f := by constructor; assumption; assumption
+  generalize fh : Γ d@ w.fst = f at *;
+  have lem := classification_lemma fJ; simp at lem; cases lem;
+  case _ h => cases h; case _ k1 k2 =>
+    have lem1 := kind_shape k2 rfl
+    have lem2 := type_shape h3 (by constructor)
+    exfalso; apply Term.is_kind_disjoint_is_type lem1 lem2
+  case _ h =>
+    cases h; case _ w h =>
+    cases h; case _ wk arrk =>
+    cases arrk; cases wk;
 
--- case lam Γ A t B ih1 ih2 =>  constructor; constructor
+case lam Γ A t B ih1 ih2 => constructor
 
--- case app Γ f A B a B' fJ aJ h0 ih1 ih2 =>
---   cases h1; case _ n ts n_stable h1 =>
---   simp at h1; rw[Option.bind_eq_some] at h1;
---   cases h1;  case _ ts' fnf =>
---   cases fnf; case _ fnf ts' =>
---   cases ts'; have h := Val.app fnf n_stable;
---   simp at *;
---   have lem := classification_lemma fJ; simp at lem;
---   cases lem;
---   case _ h => cases h
---   case _ h =>
---     cases h; case _ k h =>
---     cases h; case _ k h =>
---     cases h; case _ aK bK =>
---     have arrK := Judgment.arrow aK bK;
---     have ih := ih1 h fJ arrK (ArrowLike.arrowt); cases ih;
---     case _ h =>
---       cases h;
---       case _ => cases fnf
---       case _ => cases fnf
---     case _ h =>
---       cases h;
---       case _ h =>
---         apply Or.inr; apply Or.inl;
---         unfold ValidHeadVariable;
---         have fanf := @Term.neutral_form_app f a ts'.1 ts'.2 fnf; symm at fanf;
---         apply Exists.intro (ts'.1, ts'.snd ++ [(.term, a)]);
---         apply And.intro; assumption; simp;
---         unfold ValidHeadVariable at h; simp at h;
---         cases h; case _ h => cases h; case _ fnf' h =>
---         rw [fnf] at fnf'; cases fnf'; case _ h =>
---         cases h; simp; assumption;
---       case _ h =>
---         apply Or.inr; apply Or.inr;
---         unfold ValidHeadVariable;
---         have fanf := @Term.neutral_form_app f a ts'.1 ts'.2 fnf; symm at fanf;
---         apply Exists.intro (ts'.1, ts'.snd ++ [(.term, a)]);
---         apply And.intro; assumption; simp;
---         unfold ValidHeadVariable at h; simp at h;
---         cases h; case _ h => cases h; case _ fnf' h =>
---         rw [fnf] at fnf'; cases fnf'; case _ h =>
---         cases h; simp; assumption;
--- case _ ih1 _ =>
---   cases h1;
---   case _ h => cases h
---   case _ => constructor; constructor
+case app Γ f A B a B' fJ aJ h0 ih1 ih2 =>
+  cases h1; case _ n ts n_stable h1 =>
+  simp at h1; rw[Option.bind_eq_some] at h1;
+  cases h1;  case _ ts' fnf =>
+  cases fnf; case _ fnf hts =>
+  cases ts'; case _ x sp =>
+  simp at hts; cases hts; case _ e1 e2 =>
+  subst e1; subst e2
+  have h := Val.app x sp fnf n_stable;
+  simp at *;
+  have lem := classification_lemma fJ; simp at lem;
+  cases lem;
+  case _ h => cases h
+  case _ h =>
+    cases h; case _ k h =>
+    cases h; case _ k h =>
+    cases h; case _ aK bK =>
+    have arrK := Judgment.arrow aK bK;
+    have ih := ih1 h fJ arrK (ArrowLike.arrowt); cases ih;
+    case _ h => cases fnf
+    case _ h => cases fnf
+    case _ h =>
+      apply LambdaLike.ctor;
+      unfold ValidHeadVariable;
+      have fanf := @Term.neutral_form_app f a x sp fnf; symm at fanf;
+      apply Exists.intro (x, sp ++ [(.term, a)]);
+      apply And.intro; assumption; simp;
+      unfold ValidHeadVariable at h; simp at h;
+      cases h; case _ h => cases h; case _ fnf' h =>
+      rw [fnf] at fnf'; cases fnf'; case _ h =>
+      cases h; assumption
+    case _ h =>
+      apply LambdaLike.insttype;
+      unfold ValidHeadVariable;
+      have fanf := @Term.neutral_form_app f a x sp fnf; symm at fanf;
+      apply Exists.intro (x, sp ++ [(.term, a)]);
+      apply And.intro; assumption; simp;
+      unfold ValidHeadVariable at h; simp at h;
+      cases h; case _ h => cases h; case _ fnf' h =>
+      rw [fnf] at fnf'; cases fnf'; case _ h =>
+      cases h; assumption
+    case _ => cases fnf
+case _ ih1 _ =>
+  cases h1;
+  case _ h => cases h
+  case _ => constructor
 
--- case _ Γ f A B a B' fJ aJ _ ih1 ih2 =>
---   cases h1; case _ n ts n_stable h1 =>
---   simp at h1; rw[Option.bind_eq_some] at h1;
---   cases h1;  case _ ts' fnf =>
---   cases fnf; case _ fnf ts' =>
---   cases ts'; have h := Val.app fnf n_stable;
---   simp at *;
---   have lem := classification_lemma fJ; simp at lem;
---   cases lem;
---   case _ h => cases h
---   case _ h =>
---     cases h; case _ k h =>
---     cases h; case _ k h =>
---     cases h; case _ aK bK =>
---     have arrK := Judgment.allt aK bK;
---     have ih := ih1 h fJ arrK (ArrowLike.allt); cases ih;
---     case _ h =>
---       cases h;
---       case _ => cases fnf
---       case _ => cases fnf
---     case _ h =>
---       cases h;
---       case _ h =>
---         apply Or.inr; apply Or.inl;
---         unfold ValidHeadVariable;
---         have fanf := @Term.neutral_form_appt f a ts'.1 ts'.2 fnf; symm at fanf;
---         apply Exists.intro (ts'.1, ts'.snd ++ [(.type, a)]);
---         apply And.intro; assumption; simp;
---         unfold ValidHeadVariable at h; simp at h;
---         cases h; case _ h => cases h; case _ fnf' h =>
---         rw [fnf] at fnf'; cases fnf'; case _ h =>
---         cases h; simp; assumption;
---       case _ h =>
---         apply Or.inr; apply Or.inr;
---         unfold ValidHeadVariable;
---         have fanf := @Term.neutral_form_appt f a ts'.1 ts'.2 fnf; symm at fanf;
---         apply Exists.intro (ts'.1, ts'.snd ++ [(.type, a)]);
---         apply And.intro; assumption; simp;
---         unfold ValidHeadVariable at h; simp at h;
---         cases h; case _ h => cases h; case _ fnf' h =>
---         rw [fnf] at fnf'; cases fnf'; case _ h =>
---         cases h; simp; assumption;
--- case _ ih2 => cases h4
+case _ Γ f A B a B' fJ aJ _ ih1 ih2 =>
+  cases h1; case _ n ts n_stable h1 =>
+  simp at h1; rw[Option.bind_eq_some] at h1;
+  cases h1;  case _ ts' fnf =>
+  cases fnf; case _ fnf hts =>
+  cases ts'; case _ x sp =>
+  simp at hts; cases hts; case _ e1 e2 =>
+  subst e1; subst e2
+  have h := Val.app x sp fnf n_stable;
+  simp at *;
+  have lem := classification_lemma fJ; simp at lem;
+  cases lem;
+  case _ h => cases h
+  case _ h =>
+    cases h; case _ k h =>
+    cases h; case _ k h =>
+    cases h; case _ aK bK =>
+    have arrK := Judgment.allt aK bK;
+    have ih := ih1 h fJ arrK (ArrowLike.allt); cases ih;
+    case _ h => cases fnf
+    case _ h => cases fnf
+    case _ h =>
+        apply LambdaLike.ctor;
+        unfold ValidHeadVariable;
+        have fanf := @Term.neutral_form_appt f a x sp fnf; symm at fanf;
+        apply Exists.intro (x, sp ++ [(.type, a)]);
+        apply And.intro; assumption; simp;
+        unfold ValidHeadVariable at h; simp at h;
+        cases h; case _ h => cases h; case _ fnf' h =>
+        rw [fnf] at fnf'; cases fnf'; case _ h =>
+        cases h; assumption;
+    case _ h =>
+        apply LambdaLike.insttype;
+        unfold ValidHeadVariable;
+        have fanf := @Term.neutral_form_appt f a x sp fnf; symm at fanf;
+        apply Exists.intro (x, sp ++ [(.type, a)]);
+        apply And.intro; assumption; simp;
+        unfold ValidHeadVariable at h; simp at h;
+        cases h; case _ h => cases h; case _ fnf' h =>
+        rw [fnf] at fnf'; cases fnf'; case _ h =>
+        cases h; assumption;
+    case _ => cases fnf
+case _ ih2 => cases h4
+case choice j1 j2 j3 j4 ih1 ih2 ih3 ih4 =>
+  cases h1; case _ h => cases h
+  case _ v1 v2 =>
+    replace ih3 := ih3 v1 j3 h3 h4
+    replace ih4 := ih4 v2 j4 h3 h4
+    apply LambdaLike.choice ih3 ih4
